WIP for remove proof

src/hashtable.v
@@ -1,9 +1,10 @@
 Require Import Coq.Array.PArray.
-Require Import Coq.Init.Nat.
+Require Import Coq.Init.Nat PeanoNat.
 Require Import ZArith.
 Require Import Bool.
 Require Import Lia.
 Require Import Coq.Lists.List.
+Require Import utils Coq.ssr.ssrbool.
 Import ListNotations.
 Require Import Coq.Numbers.Cyclic.Int63.Uint63.
 
@@ -38,13 +39,42 @@ Section Hashtable.
     now case eq_spec.
   Qed.
 
-  Definition bucket := list (int * A * B).
+  Print eq_sym.
+
+  Lemma neq_sym:
+    forall (k k' : A), k <> k' -> k' <> k.
+  Proof.
+    intros k k' H. intro nH.
+    apply H. now apply eq_sym.
+  Qed.
+
+  Inductive bucket_e : Set :=
+    | C : int -> A -> B  -> bucket_e
+  .
+  Definition bucket := list (bucket_e).
   Definition table := PArray.array bucket.
   
   Record t : Set := hash_tab { 
     size : int;
     hashtab : table; 
   }.
+
+  Definition length t : int :=
+    PArray.length (hashtab t).
+
+  Fixpoint bucket_well_formed (b: bucket) (i: int) (l: int) : bool :=
+    match b with
+    | [] => true
+    | C h k _ :: b' => 
+        (hash k =? h)
+        && (i =? (h land (l - 1))) 
+        && bucket_well_formed b' i l
+    end.
+
+  Definition well_formed (h: t) : Prop :=
+    0 <? PArray.length (hashtab h) = true /\ 
+    forall i, bucket_well_formed (hashtab h).[i] i 
+              (length h) = true.
 
   Fixpoint power_2_above' (n: nat) (x p: int) {struct n} : int :=
     match n with
@@ -65,7 +95,7 @@ Section Hashtable.
     hash_tab 0 h.
 
   Definition key_index (h: t) (k: int) : int :=
-    k land PArray.length (hashtab h) - 1.
+    k mod length h.
 
   Lemma key_index_max:
     forall (h: t) (k: int),
@@ -75,31 +105,53 @@ Section Hashtable.
   Admitted.
 
   Definition get_bucket (h: t) (k: int) : bucket :=
-    if PArray.length (hashtab h) =? 0 then []
+    if length h =? 0 then []
     else (hashtab h).[key_index h k].
 
   Definition resize_heurisitic (h: t) : bool :=
-    PArray.length (hashtab h) =? 0.
+    false. 
 
-  Definition resize (h: t): t :=
-    if PArray.length (hashtab h) =? 0 then 
+  Opaque resize_heurisitic.
+
+  Definition replace_bucket (nt lt: table) (ns ls i: int) : table :=
+    fold_right (fun (e: bucket_e) a =>
+      let (h, k, v) := e in
+      if i =? h mod ls then
+        a.[h mod ns <- e :: a.[h mod ns]]
+      else a) 
+    nt lt.[i].
+
+  Definition copy_tab (ht: t) (i: int) : t :=
+    let last_size := length ht in
+    let new_size := last_size * 2 in
+    let a := make new_size [] in
+    let new_tab := 
+      fold_int (fun i a =>
+        replace_bucket a (hashtab ht) (PArray.length a) (length ht) i) 
+      i a 
+    in
+    hash_tab (size ht) new_tab.
+
+  Definition resize (ht: t): t :=
+    if length ht =? 0 then 
       hash_tab 0 (make 16 [])
-    else h.
+    else if resize_heurisitic ht then
+      copy_tab ht (length ht)
+    else ht.
 
   Lemma length_resize:
     forall (h: t),
-    (0 < to_Z (PArray.length (hashtab (resize h))))%Z.
+    (0 < to_Z (length (resize h)))%Z.
   Proof.
     admit.
   Admitted.
 
   Lemma length_resize_non_neg:
     forall (h: t),
-    (PArray.length (hashtab (resize h))) <> 0.
+    (length (resize h)) <> 0.
   Proof.
     admit.
   Admitted.
-
 
   Definition add (h: t) (key: A) (v: B) : t :=
     let h := resize h in
@@ -107,13 +159,13 @@ Section Hashtable.
     let hash := hash key in
     let i := key_index h hash in
     let bucket := get tab i in
-    let new := (hash, key, v) :: tab.[i] in
+    let new := C hash key v :: tab.[i] in
     hash_tab (size h + 1) tab.[i<-new].
 
   Fixpoint find_rec (l: bucket) (h: int) (k: A): option B :=
     match l with
     | [] => None
-    | (h', k', v) :: l' => 
+    | C h' k' v :: l' => 
         if andb (h =? h') (eq k k')
         then Some v 
         else find_rec l' h k
@@ -122,7 +174,7 @@ Section Hashtable.
   Fixpoint find_all_rec (l: bucket) (h: int) (k: A) (acc: list B): list B :=
     match l with
     | [] => List.rev' acc
-    | (h', k', v) :: l' => 
+    | C h' k' v :: l' => 
         if andb (h =? h') (eq k k')
         then find_all_rec l' h k (v :: acc)
         else find_all_rec l' h k acc
@@ -131,21 +183,20 @@ Section Hashtable.
   Fixpoint find_all_rec' (l: bucket) (h: int) (k: A) : list B :=
     match l with
     | [] => []
-    | (h', k', v) :: l' => 
+    | C h' k' v :: l' => 
         if andb (h =? h') (eq k k')
         then v :: find_all_rec' l' h k
         else find_all_rec' l' h k
     end.
 
   Lemma find_all_rec_correct:
-    forall (l: bucket) (h: int) (key: A),
-    find_all_rec l h key [] = find_all_rec' l h key.
+    forall (l: bucket) (h: int) (key: A) acc,
+    find_all_rec l h key acc = rev acc ++ find_all_rec' l h key.
   Proof.
     intros l h k. 
-    change (find_all_rec l h k [] = rev [] ++ find_all_rec' l h k).
-    generalize (nil : list B). induction l.
+    induction l.
     + intros acc. simpl. apply rev_append_rev.
-    + intros acc. simpl. destruct a, p. case (_ && _).
+    + intros acc. simpl. destruct a. case (_ && _).
       rewrite IHl. simpl. rewrite <- app_assoc. easy.
       apply IHl.
   Qed.
@@ -159,15 +210,194 @@ Section Hashtable.
     let hash := hash key in
     find_all_rec (get_bucket h hash) hash key [].
 
+  Lemma mult_size_non_neg:
+    forall (ht: t), 
+    PArray.length (hashtab ht) =? 0 = false ->
+    PArray.length (hashtab ht) * 2 =? 0 = false.
+  Proof.
+    intros ht H.
+    case (eqbP (PArray.length (hashtab ht)) 0) as [|H'] in H; try discriminate.
+    rewrite eqb_false_spec. intro Hd. apply H'.
+    case (eqbP (PArray.length (hashtab ht) * 2) 0) as [Hd'|Hd'] in Hd;
+    rewrite mul_spec in Hd'; change (to_Z 2) with 2%Z in Hd';
+    change (to_Z 0) with 0%Z in *. 
+  Admitted.
+
+  Lemma replace_bucket_length:
+    forall (nt lt: table) i,
+    PArray.length (replace_bucket nt lt (PArray.length nt) (PArray.length lt) i) 
+    = PArray.length nt.
+  Proof.
+    intros nt lt i.
+    unfold replace_bucket.
+    induction lt.[i]; simpl.
+    + easy.
+    + destruct a.
+      case (i =? _ mod (PArray.length lt)); [rewrite length_set|]; apply IHb.
+  Qed.
+
+  Lemma copy_tab_lenght:
+    forall (ht: t) (i: int),
+    length ht =? 0 = false ->
+    length (copy_tab ht i) =? 0 = false.
+  Proof.
+    intros ht i H.
+    unfold copy_tab, length. simpl.
+    rewrite fold_int_spec.
+    induction (Z.to_nat (to_Z i)).
+    + simpl. rewrite length_make.
+      case (_ <=? _).
+      - now apply mult_size_non_neg.
+      - reflexivity.
+    + simpl.
+      rewrite replace_bucket_length.
+      apply IHn.
+  Qed.
+
+  Lemma fold_right_length:
+    forall nt lt i0 i b,
+    (PArray.length nt =? 0) = false ->
+    (i0 mod PArray.length nt <?
+      PArray.length
+       (fold_right
+          (fun (e : bucket_e) (a0 : array (list bucket_e)) =>
+           let (h, _, _) := e in
+           if i =? h mod PArray.length (hashtab lt)
+           then a0.[h mod PArray.length nt<-e :: a0.[h mod PArray.length nt]]
+           else a0) nt b)) = true.
+  Proof.
+    intros nt lt i0 i b H.
+    induction b. simpl. rewrite ltb_spec, mod_spec.
+    apply Z.mod_pos_bound. generalize (to_Z_bounded (PArray.length nt)).
+    case (eqbP (PArray.length nt) 0) as [| H'] in H; try discriminate.
+    change (to_Z 0) with 0%Z in H'.
+    change (list bucket_e) with bucket in *. lia.
+    simpl. destruct a. case (i =? _). 2: apply IHb.
+    rewrite PArray.length_set. apply IHb.
+  Qed.
+
+  Lemma replace_bucket_correct1:
+    forall (nt: table) (lt: t) (k: A) (i s: int),
+    length lt =? 0 = false ->
+    PArray.length nt =? 0 = false ->
+    i = (hash k) mod (length lt) ->
+    find_all (hash_tab s nt) k = [] ->
+    find_all (hash_tab s (replace_bucket nt (hashtab lt)
+                            (PArray.length nt) (length lt) i)) k =
+    find_all lt k.
+  Proof.
+    intros nt lt j i s Hlt Hnt H Hf.
+    unfold find_all, get_bucket, key_index, length.
+    simpl. rewrite replace_bucket_length. rewrite Hnt.
+    unfold length in Hlt. rewrite Hlt.
+    unfold replace_bucket. unfold length in *.
+    rewrite <- H.
+    induction (hashtab lt).[i].
+    - simpl. unfold find_all in Hf.
+      unfold get_bucket in Hf. unfold key_index, length in Hf. simpl in Hf.
+      rewrite Hnt in Hf.
+      rewrite Hf. now simpl.
+    - simpl. destruct a.
+      case (i =? i0 mod PArray.length (hashtab lt)) eqn:Heq.
+      + case (hash j =? i0) eqn:Hj.
+        * rewrite eqb_spec in Hj. rewrite Hj.
+          rewrite get_set_same. simpl. rewrite eqb_refl, andb_true_l.
+          case (eq j a); rewrite 2!find_all_rec_correct in IHb; simpl in IHb;
+          rewrite 2!find_all_rec_correct; apply f_equal;
+          rewrite <- Hj; apply IHb. now apply fold_right_length.
+        * simpl.
+          case (i0 mod PArray.length nt =? hash j mod PArray.length nt) eqn:Hheq.
+          **rewrite eqb_spec in Hheq. rewrite Hheq, get_set_same.
+            rewrite 2!find_all_rec_correct. simpl. rewrite Hj. simpl.
+            rewrite 2!find_all_rec_correct in IHb. simpl in IHb. apply IHb.
+            now apply fold_right_length.
+          **rewrite get_set_other. apply IHb. now rewrite eqb_false_spec in Hheq.
+      + rewrite IHb. rewrite H in Heq.
+        case (eqbP (hash j mod PArray.length (hashtab lt)) 
+                (i0 mod PArray.length (hashtab lt))) as [|Heq']in Heq.
+        try discriminate.
+        rewrite 2!mod_spec in Heq'.
+        assert (to_Z (hash j) <> to_Z i0) by (intros H'; now rewrite H' in Heq').
+        now case (eqbP (hash j) i0).
+  Qed.
+
+  Lemma replace_bucket_correct2:
+    forall (nt: table) (lt: t) (k: A) (i s: int),
+    length lt =? 0 = false ->
+    PArray.length nt =? 0 = false ->
+    i <> (hash k) mod (length lt) ->
+    (to_Z (length lt) <= to_Z (PArray.length nt))%Z -> 
+    find_all (hash_tab s (replace_bucket nt (hashtab lt)
+                            (PArray.length nt) (length lt) i)) k =
+    find_all (hash_tab s nt) k.
+  Proof.
+    intros nt lt j i s Hlt Hnt H Hf.
+    unfold find_all, get_bucket, key_index, length.
+    simpl. rewrite replace_bucket_length. rewrite Hnt.
+    unfold replace_bucket. unfold length in *.
+    induction (hashtab lt).[i]. now simpl.
+    simpl. destruct a. case (i =? i0 mod (PArray.length (hashtab lt))) eqn:Heq.
+    2: apply IHb.
+    case (i0 mod PArray.length nt =? hash j mod PArray.length nt) eqn:Hm.
+    + rewrite eqb_spec in Hm. rewrite Hm. rewrite get_set_same.
+      rewrite find_all_rec_correct. simpl.
+      assert (Hd: hash j <> i0). 
+      { rewrite eqb_spec in Heq. rewrite Heq in H.
+        intros Hd. rewrite Hd in H. now apply H. }
+      rewrite <- eqb_false_spec in Hd. rewrite Hd. simpl.
+      rewrite find_all_rec_correct in IHb. simpl in IHb. exact IHb.
+      now apply fold_right_length.
+    + rewrite get_set_other. exact IHb. now rewrite eqb_false_spec in Hm.
+  Qed.
+
+  Lemma copy_tab_correct:
+    forall (ht: t) (k: A) (i: int),
+      length ht =? 0 = false ->
+      (hash k) mod length ht <? i = true -> 
+      find_all (copy_tab ht i) k = find_all ht k.
+  Proof.
+    intros ht k i H. unfold length. rewrite ltb_spec. rewrite Z2Nat.inj_lt.
+    2: generalize (to_Z_bounded (hash k mod PArray.length (hashtab ht))); lia.
+    2: generalize (to_Z_bounded i); lia.
+    unfold copy_tab. rewrite fold_int_spec.
+    induction (Z.to_nat (to_Z i)).
+    + generalize (to_Z_bounded (hash k)). intros Hb.
+      rewrite mod_spec, Z2Nat.inj_mod. lia. easy.
+      generalize (to_Z_bounded (PArray.length (hashtab ht))).
+      now intros Hb'.
+    + case (Z.to_nat φ (hash k mod PArray.length (hashtab ht)) <? n)%nat eqn:Hn.
+      - simpl. intros _. rewrite replace_bucket_correct'. apply IHn.
+        now rewrite Nat.ltb_lt in Hn.
+        induction n. simpl. rewrite length_make.
+        * case (_ <=? max_length). 2: apply leb_length.
+          rewrite leb_spec, mul_spec. change (to_Z 2) with 2%Z.
+          rewrite Z.mod_small. generalize (to_Z_bounded (length ht)). lia.
+          split. generalize (to_Z_bounded (length ht)). lia.
+          apply Z.le_lt_trans with (m:=(to_Z PArray.max_length * 2)%Z).
+          unfold length. apply Zmult_le_compat_r.
+          rewrite <- leb_spec. apply leb_length. lia. cbn. easy.
+        * simpl. admit.
+      - simpl. intro H0. apply replace_bucket_correct. admit.
+  Qed.
+
   Lemma find_all_resize:
     forall (h: t) (k: A),
     find_all (resize h) k = find_all h k.
   Proof.
-    intros h k. unfold resize, find_all, get_bucket.
+    intros h k.
     case (PArray.length (hashtab h) =? 0) eqn:Heqb.
-    simpl eqb. cbn iota. unfold hashtab.
-    now rewrite get_make.
-    now rewrite Heqb.
+    - unfold resize, find_all, get_bucket.
+      rewrite Heqb.
+      set (x:=make 16 []). simpl. unfold x.
+      now rewrite get_make.
+    - unfold resize. rewrite Heqb.
+      case resize_heurisitic. 2: reflexivity.
+      apply find_all_copy_tab.
+      rewrite ltb_spec, mod_spec.
+      apply Z.mod_pos_bound.
+      generalize (to_Z_bounded (PArray.length (hashtab h))).
+      destruct (eqbP (PArray.length (hashtab h)) 0). discriminate.
+      rewrite to_Z_0 in n. lia.
   Qed.
 
   Theorem hempty:
@@ -189,7 +419,7 @@ Section Hashtable.
     now rewrite H.
   Qed.
 
-  Theorem dadd:
+  Theorem find_add_same:
     forall (k: A) (v: B) (h: t),
     find_all (add h k v) k = v :: (find_all h k).
   Proof.
@@ -206,6 +436,44 @@ Section Hashtable.
     2:unfold add; simpl; rewrite length_set.
     all:apply length_resize_non_neg.
   Qed.
+
+  Theorem find_add_diff:
+    forall (k k': A) (v: B) (h: t),
+    k <> k' -> find_all (add h k v) k' = find_all h k'.
+  Proof.
+    intros k k' v h Hdiff.
+    unfold add, find_all, get_bucket. simpl.
+    rewrite length_set.
+    rewrite eqb_false_complete; [|apply length_resize_non_neg].
+    case (PArray.length (hashtab h) =? 0) eqn:H.
+    + unfold resize, key_index. rewrite H. set (m:=make 16 []).
+      simpl.
+      rewrite length_set. simpl.
+      case (hash k' land 15 =? hash k land 15) eqn:Hhk.
+      - apply eqb_correct in Hhk.
+        rewrite Hhk, get_set_same. simpl.
+        rewrite eq_false. 
+        assert ((hash k' =? hash k) && false = false).
+        apply andb_false_iff; now right.
+        rewrite H0. unfold m. rewrite get_make. now simpl.
+        now apply neq_sym.
+        rewrite ltb_spec. unfold m. simpl. admit.
+      - unfold m. rewrite get_make, get_set_other.
+        rewrite get_make. now simpl.
+        rewrite  eqb_false_spec in Hhk.
+        intro Hd. apply eq_sym in Hd.
+        now apply Hhk.
+    + unfold resize, key_index. rewrite H. simpl.
+      rewrite length_set.
+      case (hash k land (PArray.length (hashtab h) - 1) =? 
+            hash k' land (PArray.length (hashtab h) - 1)) eqn:Heq.
+      - apply eqb_spec in Heq. rewrite Heq, get_set_same. simpl.
+        rewrite eq_false; [|now apply neq_sym].
+        assert ((hash k' =? hash k) && false = false).
+        apply andb_false_iff; now right.
+        rewrite H0. easy. admit.
+      - apply eqb_false_spec in Heq. rewrite get_set_other. easy. easy.
+  Admitted.
 
 End Hashtable.
 
@@ -224,7 +492,7 @@ Module HashTable (T: Hash_type).
   Definition add {B: Set} (h: t B) (key: T.A) (v: B) :=
     add T.hash h key v.
 
-  Definition find {B: Set} (h: t B) (key: T.A): option B :=
-    find T.eq T.hash key h.
+  (* Definition find {B: Set} (h: t B) (key: T.A): option B := *)
+  (*   find T.eq T.hash key h. *)
 End HashTable.
 
