src/utils.v
@@ -1,4 +1,9 @@
 Require Import Coq.Lists.List.
+Require Import ZArith.
+Require Import Lia.
+Require Import Coq.Numbers.Cyclic.Int63.Uint63.
+Open Scope uint63_scope.
+
 Import ListNotations.
 
 Section List.
@@ -13,4 +18,116 @@ Section List.
 End List.
 
 Arguments find_snd : clear implicits.
+
+Lemma add_neutral:
+  forall (u: int), u + 0 = u.
+Proof.
+  intros u. rewrite <- of_to_Z at 1.
+  rewrite add_spec. change (to_Z 0) with 0%Z.
+  rewrite Z.add_0_r. rewrite Z.mod_small.
+  apply of_to_Z.
+  generalize (to_Z_bounded u). lia.
+Qed.
+
+Lemma of_Z_add:
+  forall (u v: Z), of_Z (u + v)%Z = of_Z u + of_Z v.
+Proof.
+  intros u v. unfold of_Z. case u, v; simpl; try easy.
+  now rewrite add_comm, add_neutral.
+  now rewrite add_comm, add_neutral.
+  now rewrite add_neutral.
+  admit.
+  admit.
+  now rewrite add_neutral.
+  admit.
+  admit.
+Admitted.
+
+Lemma fold_int_aux:
+  forall (i e: int), i <? e = true-> i <? i + 1 = true.
+Proof.
+  intros i e H.
+  apply ltb_spec. rewrite add_spec.
+  rewrite Z.mod_small. apply Z.lt_succ_diag_r.
+  apply ltb_spec in H.
+  generalize (to_Z_bounded e) (to_Z_bounded i). change (to_Z 1) with 1%Z.
+  lia.
+Qed.
+
+
+Definition fold_int' (T: Type) (f : int -> T -> T) 
+                     (e: int) (acc: T) 
+                     (H: Acc (fun x y => y <? x = true) 0 ): T.
+Proof.
+  revert acc H.
+  generalize 0.
+  fix cont 3.
+  intros i acc H.
+  case (i <? e) eqn:Hlt. 2: exact acc.
+  apply (cont (i+1) (f i acc)).
+  case H. intros H0. apply H0. apply (fold_int_aux _ _ Hlt).
+Defined.
+
+Print fold_int'.
+
+Lemma acc_int:
+  forall x, Acc (fun x y => y <? x = true) x.
+Proof.
+  assert (H: forall y, of_Z (wB - 1 - (wB - 1 - to_Z y)) = y).
+  { intros y.
+    rewrite <- (of_to_Z y) at 2.
+    apply f_equal. ring. }
+  intros x.
+  rewrite <- H.
+  apply (Z_lt_induction 
+          (fun x => to_Z (of_Z x) = x -> 
+          Acc (fun x y : int => (y <? x) = true) (of_Z (wB - 1 - x)))).
+  clear x.
+  intros x IHn Hpos.
+  apply Acc_intro.
+  intros y Heq.
+  rewrite <- H.
+  apply IHn. split.
+  generalize (to_Z_bounded y). lia.
+  apply ltb_spec in Heq.
+  rewrite of_Z_spec, Z.mod_small in Heq. lia.
+  rewrite <- Hpos.
+  generalize (to_Z_bounded (of_Z x)). lia.
+  rewrite of_Z_spec. apply Z.mod_small.
+  generalize (to_Z_bounded y). lia.
+  generalize (to_Z_bounded x). lia.
+  rewrite of_Z_spec. apply Z.mod_small.
+  generalize (to_Z_bounded x). lia.
+Qed.
+
+Definition fold_int {T: Type} (f : int -> T -> T) (e: int) (acc: T) :=
+  fold_int' T f e acc (Acc_intro_generator 22 acc_int 0).
+
+Lemma fold_int_spec :
+  forall T (f : int -> T -> T) e acc,
+  fold_int f e acc =
+  nat_rect (fun _ => T) acc 
+           (fun n acc => f (of_Z (Z.of_nat n)) acc)
+           (Z.to_nat (to_Z e)).
+Proof.
+  intros T f e.
+  pattern e at 1.
+  elim of_to_Z.
+  generalize (proj2 (to_Z_bounded e)).
+  pattern (to_Z e) at 1 2.
+  elim Z2Nat.id. 2: apply to_Z_bounded.
+  induction (Z.to_nat (to_Z e)).
+  easy.
+  rewrite Nat2Z.inj_succ.
+  unfold Z.succ. intros Hs.
+  rewrite of_Z_add. change (of_Z 1) with 1. simpl.
+Admitted.
+
+Definition v := fold_int (fun n acc => n :: acc ) 3 [].
+
+Compute v.
+
+Definition v' := nat_rect _ [] (fun n acc => of_Z (Z.of_nat n) :: acc ) 3.
+
+Compute v'.
 
